Greedy.thy
@@ -52,16 +52,17 @@ text "The weight of a set of elements: for simplicity's sake we assume that
 definition "weight (w :: 'a \<Rightarrow> int) A = (\<Sum>x\<in>A. w x)" 
 definition "neg (w :: 'a \<Rightarrow> int) = (\<lambda>x. - w x)"
 
-lemma Sorted_neg :
-"Sorted (neg w) xs = Sorted w (rev xs)"
-  by(induct_tac xs, (simp add: neg_def Sorted_append)+)
+lemma sorted_by_neg :
+"sorted_by (neg w) xs = sorted_by w (rev xs)"
+  by(induct xs, (fastforce simp add: sorted_by_def neg_def sorted_wrt_append)+)
+
 
 lemma weight0 :
 "weight w {} = 0"
   by(simp add: weight_def)
 
 lemma weight_neg :
-"weight (neg w) S = -(weight w S)"
+"weight (neg w) S = -weight w S"
   by(simp add: weight_def neg_def, rule sum_negf)
 
 lemma weight_mono :
@@ -90,7 +91,7 @@ begin
 definition "basis G X = (finite G \<and> X \<in> \<I> \<and> X \<subseteq> G \<and> (\<forall>X'. X' \<subseteq> G \<longrightarrow> X' \<in> \<I> \<longrightarrow> card X' \<le> card X))"
 
 
-text "We can thus define maximum and minimum weight bases"
+text "maximum/minimum weight bases"
 definition "max_weight_basis w G X = (basis G X \<and> (\<forall>B. basis G B \<longrightarrow> weight w B \<le> weight w X))"
 definition "min_weight_basis w G X = (basis G X \<and> (\<forall>B. basis G B \<longrightarrow> weight w B \<ge> weight w X))"
 
@@ -119,16 +120,16 @@ lemma basis_ext :
        apply(erule finite_subset, assumption)+
      apply assumption+
    apply clarify
-   apply(drule_tac x="{e} \<union> A" in spec)
-   apply (metis card_insert_disjoint card_seteq diff_less_mono2 finite_subset insert_is_Un insert_subset lessI not_le_imp_less subsetD)
+   apply(drule_tac x="{e} \<union> A" in spec, simp)
+   apply (metis card_seteq diff_less_mono2 finite_insert insertCI leI rev_finite_subset subset_iff)
   apply (metis basis_def not_le_imp_less)
   done
 
 
 subsection "The duality between maximum and minimum weight bases"
 
-lemma MaxWeightBasis_neg :
-  "max_weight_basis (neg w) G X = min_weight_basis w G X"
+lemma max_weight_basis_neg :
+"max_weight_basis (neg w) G X = min_weight_basis w G X"
   unfolding max_weight_basis_def min_weight_basis_def
   by (metis neg_le_iff_le weight_neg)
 
@@ -224,7 +225,7 @@ end (* the finite matroids locale *)
 section "A greedy tactic for lists with weighted elements"
 
 
-locale language_struct =
+locale language =
   fixes \<L> :: "'a list set"
   assumes \<L>_prop : "xs \<in> \<L> \<Longrightarrow> set xs = set xs' \<Longrightarrow> distinct xs \<Longrightarrow> distinct xs' \<Longrightarrow> 
                     xs' \<in> \<L>"
@@ -236,25 +237,22 @@ definition \<L>_img :: "'a set set"
 
 lemma \<L>_img_eq :
 "distinct xs \<Longrightarrow> (set xs \<in> \<L>_img) = (xs \<in> \<L>)"
-  apply(simp add: \<L>_img_def)
-  apply(rule iffI)
-   apply clarify
-   apply(erule \<L>_prop)
-  by fastforce+
+  using \<L>_img_def \<L>_prop by fastforce
 
-end
+end (* language locale *)
 
 
 
-locale greedy_tactic = language_struct +
+locale greedy_tactic = language +
   fixes w :: "'a \<Rightarrow> int" 
   assumes \<L>_img_independence : "Independent \<L>_img"
 begin
 
-text "In addition to the language-struct locale we assume that the elements of type @{typ 'a} 
-      are weighted by the function @{term w}
-      and that @{term \<L>_img} forms a family of independent sets so we can interpret the finite 
-      matroids locale in this context."
+text "In addition to the language locale we have assumed that 
+        (i)  the elements of type @{typ 'a} are weighted by the function @{term w}
+        (ii) @{term \<L>_img} forms a family of independent sets 
+
+      and can interpret the finite matroids locale in this context:"
 interpretation fm : finite_matroids \<L>_img
   by(unfold_locales, rule \<L>_img_independence)
 
@@ -341,8 +339,8 @@ theorem prefixed_point_property :
 
 text "applying the divide-and-conquer synthesis rule:" 
 interpretation greedy: DaC_synthesis 
-"{(xs, set xs) |xs. distinct xs \<and> Sorted w xs}"                 (* \<alpha>\<^sub>1 *)
-"{(xs, set xs) |xs. distinct xs}"                               (* \<alpha>\<^sub>2 *)
+"{(xs, set xs) |xs. distinct xs \<and> sorted_by w xs}"                 (* \<alpha>\<^sub>1 *)
+"{(xs, set xs) |xs. distinct xs}"                                  (* \<alpha>\<^sub>2 *)
 greedy_spec decomp_spec comp_spec decomp_impl comp_impl
   apply(unfold_locales)
      apply(rule prefixed_point_property)
@@ -353,7 +351,7 @@ greedy_spec decomp_spec comp_spec decomp_impl comp_impl
      apply(rule_tac b=Empty in relcompI, clarsimp+)
     apply(rename_tac x xs)
     apply(rule_tac b="Dcmp x (set xs)" in relcompI)
-     apply simp+
+     apply(simp add: sorted_by_def)+
 
   text "composition implementation:"
    apply(clarsimp simp: comp_spec_def comp_impl_def graph_of_def Relt_def)
@@ -405,6 +403,7 @@ lemma syn_greedy_eqs[simp] :
 "syn_greedy (x#xs) = (if x # syn_greedy xs \<in> \<L> then x # syn_greedy xs else syn_greedy xs)"
 unfolding syn_greedy_def by(subst greedy.dac_unfold, simp add: decomp_impl_def comp_impl_def ReltF_eqs)+
 
+
 lemma syn_greedy_sub[simp] :
 "set(syn_greedy xs) \<subseteq> set xs"
   by(induct xs, simp+, fast)
@@ -418,7 +417,7 @@ lemma syn_greedy_dist :
 
 
 lemma syn_greedy_max_basis :
-"distinct xs \<Longrightarrow> Sorted w xs \<Longrightarrow> 
+"distinct xs \<Longrightarrow> sorted_by w xs \<Longrightarrow> 
  max_weight_basis w (set xs) (set(syn_greedy xs))"
   apply(insert greedy.dac_impl)
   apply(drule_tac c="(set xs, set(syn_greedy xs))" in subsetD)
@@ -441,7 +440,7 @@ locale enhanced_greedy = greedy_tactic +
      and  transl  : "distinct xs \<Longrightarrow> (foldr ins xs [] \<in> \<L>') = (xs \<in> \<L>)"
 begin
 
-subsection "First transformation step"
+subsection "The first transformation step"
 
 fun greedy where
   "greedy [] = []"
@@ -476,7 +475,7 @@ lemma transformation1_correctness :
   by(simp add: ins_gen)
 
 
-subsection "Second transformation (tail-recursion)"
+subsection "The second transformation (tail-recursion)"
 
 
 fun greedy_tr 
@@ -509,14 +508,14 @@ lemma greedy_greedy_tr' :
 
 text "Summarising the main result of the greedy tactic (synthesis + transformations): "
 corollary greedy_tr_max_basis :
- "distinct xs \<Longrightarrow> Sorted (neg w) xs \<Longrightarrow> 
-  max_weight_basis w (set xs) (set(greedy_tr xs []))"
+"distinct xs \<Longrightarrow> sorted_by (neg w) xs \<Longrightarrow> 
+ max_weight_basis w (set xs) (set(greedy_tr xs []))"
   apply(subst transformation2_correctness[THEN sym])
   apply(subst transformation1_correctness, simp)
   apply(subst set_rev[THEN sym])
   apply(rule syn_greedy_max_basis)
   apply simp
-  apply(subst Sorted_neg[THEN sym])
+  apply(subst sorted_by_neg[THEN sym])
   apply assumption+
   done
 
